WIP

Risc0/Gadgets/ComputeDecode/Constraints/WeakestPresPart0.lean
@@ -1,32 +1,63 @@
 import Risc0.Basic
 import Risc0.MlirTactics
-import Risc0.Gadgets.ComputeDecode.Constraints.Code
+import Risc0.Gadgets.ComputeDecode.Constraints.CodeDrops
 
 namespace Risc0.ComputeDecode.Constraints.WP
 
 open MLIRNotation
 
 -- The state obtained by running Code.part0 on st
-def part0_state (st : State) : State :=
+def part0_state (st: State) : State :=
   
-        ((((st[felts][{ name := "%0" }] ← 128)[felts][{ name := "%1" }] ← 16)[felts][{ name := "%2" }] ←
-            8)[felts][{ name := "%3" }] ←
-          2) 
+        ((((st[props][{ name := "%6" }] ← True)[felts][{ name := "%4" }] ← 4)["%13"] ←ₛ
+            getImpl st { name := "data" } 0 8)[felts][{ name := "%14" }] ←
+          Option.get!
+              (State.felts
+                (((st[props][{ name := "%6" }] ← True)[felts][{ name := "%4" }] ← 4)["%13"] ←ₛ
+                  getImpl st { name := "data" } 0 8)
+                { name := "%13" }) *
+            4) 
+
+def part0_drops (st: State) : State :=
+  State.dropFelts (st) ⟨"%13"⟩
 
 -- Run the whole program by using part0_state rather than Code.part0
-def part0_state_update (st : State) : State :=
-  Γ (part0_state st) ⟦Code.part1; Code.part2; Code.part3; Code.part4; Code.part5; Code.part6; Code.part7; Code.part8; Code.part9; Code.part10; Code.part11; Code.part12; Code.part13; Code.part14; Code.part15; Code.part16⟧
+def part0_state_update (st: State): State :=
+  Γ (part0_drops (part0_state st)) ⟦Code.part1;dropfelt ⟨"%15"⟩;Code.part2;dropfelt ⟨"%14"⟩;dropfelt ⟨"%16"⟩;dropfelt ⟨"%17"⟩;dropfelt ⟨"%18"⟩;dropfelt ⟨"%19"⟩;Code.part3;dropfelt ⟨"%20"⟩;dropfelt ⟨"%12"⟩;Code.part4;dropfelt ⟨"%21"⟩;dropfelt ⟨"%5"⟩;dropfelt ⟨"%22"⟩;dropfelt ⟨"%23"⟩;dropfelt ⟨"%24"⟩;Code.part5;dropfelt ⟨"%25"⟩;dropfelt ⟨"%11"⟩;dropfelt ⟨"%26"⟩;dropfelt ⟨"%10"⟩;Code.part6;dropfelt ⟨"%27"⟩;dropfelt ⟨"%30"⟩;Code.part7;dropfelt ⟨"%2"⟩;dropfelt ⟨"%3"⟩;dropfelt ⟨"%33"⟩;dropfelt ⟨"%34"⟩;dropfelt ⟨"%35"⟩;dropfelt ⟨"%36"⟩;Code.part8;dropfelt ⟨"%31"⟩;dropfelt ⟨"%37"⟩;dropfelt ⟨"%32"⟩;dropfelt ⟨"%38"⟩;dropfelt ⟨"%39"⟩;Code.part9;dropfelt ⟨"%40"⟩;dropfelt ⟨"%29"⟩;dropfelt ⟨"%41"⟩;dropfelt ⟨"%9"⟩;Code.part10;dropfelt ⟨"%42"⟩;dropfelt ⟨"%45"⟩;Code.part11;dropfelt ⟨"%4"⟩;dropfelt ⟨"%1"⟩;dropfelt ⟨"%48"⟩;dropfelt ⟨"%49"⟩;dropfelt ⟨"%47"⟩;dropfelt ⟨"%50"⟩;Code.part12;dropfelt ⟨"%51"⟩;dropfelt ⟨"%52"⟩;dropfelt ⟨"%53"⟩;Code.part13;dropfelt ⟨"%46"⟩;dropfelt ⟨"%54"⟩;dropfelt ⟨"%55"⟩;dropfelt ⟨"%44"⟩;Code.part14;dropfelt ⟨"%0"⟩;dropfelt ⟨"%56"⟩;dropfelt ⟨"%8"⟩;dropfelt ⟨"%57"⟩;dropfelt ⟨"%60"⟩;Code.part15;dropfelt ⟨"%61"⟩;dropfelt ⟨"%59"⟩;dropfelt ⟨"%62"⟩;dropfelt ⟨"%7"⟩;Code.part16;dropfelt ⟨"%6"⟩;dropfelt ⟨"%28"⟩;dropfelt ⟨"%43"⟩;dropfelt ⟨"%58"⟩;dropfelt ⟨"%63"⟩;dropfelt ⟨"%64"⟩⟧
 
 -- Prove that substituting part0_state for Code.part0 produces the same result
 lemma part0_wp {st : State} :
-  Code.run st ↔
+  Code.getReturn (Γ st ⟦Code.part0;dropfelt ⟨"%13"⟩;Code.part1;dropfelt ⟨"%15"⟩;Code.part2;dropfelt ⟨"%14"⟩;dropfelt ⟨"%16"⟩;dropfelt ⟨"%17"⟩;dropfelt ⟨"%18"⟩;dropfelt ⟨"%19"⟩;Code.part3;dropfelt ⟨"%20"⟩;dropfelt ⟨"%12"⟩;Code.part4;dropfelt ⟨"%21"⟩;dropfelt ⟨"%5"⟩;dropfelt ⟨"%22"⟩;dropfelt ⟨"%23"⟩;dropfelt ⟨"%24"⟩;Code.part5;dropfelt ⟨"%25"⟩;dropfelt ⟨"%11"⟩;dropfelt ⟨"%26"⟩;dropfelt ⟨"%10"⟩;Code.part6;dropfelt ⟨"%27"⟩;dropfelt ⟨"%30"⟩;Code.part7;dropfelt ⟨"%2"⟩;dropfelt ⟨"%3"⟩;dropfelt ⟨"%33"⟩;dropfelt ⟨"%34"⟩;dropfelt ⟨"%35"⟩;dropfelt ⟨"%36"⟩;Code.part8;dropfelt ⟨"%31"⟩;dropfelt ⟨"%37"⟩;dropfelt ⟨"%32"⟩;dropfelt ⟨"%38"⟩;dropfelt ⟨"%39"⟩;Code.part9;dropfelt ⟨"%40"⟩;dropfelt ⟨"%29"⟩;dropfelt ⟨"%41"⟩;dropfelt ⟨"%9"⟩;Code.part10;dropfelt ⟨"%42"⟩;dropfelt ⟨"%45"⟩;Code.part11;dropfelt ⟨"%4"⟩;dropfelt ⟨"%1"⟩;dropfelt ⟨"%48"⟩;dropfelt ⟨"%49"⟩;dropfelt ⟨"%47"⟩;dropfelt ⟨"%50"⟩;Code.part12;dropfelt ⟨"%51"⟩;dropfelt ⟨"%52"⟩;dropfelt ⟨"%53"⟩;Code.part13;dropfelt ⟨"%46"⟩;dropfelt ⟨"%54"⟩;dropfelt ⟨"%55"⟩;dropfelt ⟨"%44"⟩;Code.part14;dropfelt ⟨"%0"⟩;dropfelt ⟨"%56"⟩;dropfelt ⟨"%8"⟩;dropfelt ⟨"%57"⟩;dropfelt ⟨"%60"⟩;Code.part15;dropfelt ⟨"%61"⟩;dropfelt ⟨"%59"⟩;dropfelt ⟨"%62"⟩;dropfelt ⟨"%7"⟩;Code.part16;dropfelt ⟨"%6"⟩;dropfelt ⟨"%28"⟩;dropfelt ⟨"%43"⟩;dropfelt ⟨"%58"⟩;dropfelt ⟨"%63"⟩;dropfelt ⟨"%64"⟩⟧)↔
   Code.getReturn (part0_state_update st) := by
-    unfold Code.run MLIR.runProgram; simp only
-    rewrite [←Code.parts_combine]; unfold Code.parts_combined
-    generalize eq : (Code.part1; Code.part2; Code.part3; Code.part4; Code.part5; Code.part6; Code.part7; Code.part8; Code.part9; Code.part10; Code.part11; Code.part12; Code.part13; Code.part14; Code.part15; Code.part16) = prog
-    unfold Code.part0
-    MLIR
-    unfold part0_state_update part0_state
-    rw [←eq]
+  generalize eq : (dropfelt ⟨"%13"⟩;Code.part1;dropfelt ⟨"%15"⟩;Code.part2;dropfelt ⟨"%14"⟩;dropfelt ⟨"%16"⟩;dropfelt ⟨"%17"⟩;dropfelt ⟨"%18"⟩;dropfelt ⟨"%19"⟩;Code.part3;dropfelt ⟨"%20"⟩;dropfelt ⟨"%12"⟩;Code.part4;dropfelt ⟨"%21"⟩;dropfelt ⟨"%5"⟩;dropfelt ⟨"%22"⟩;dropfelt ⟨"%23"⟩;dropfelt ⟨"%24"⟩;Code.part5;dropfelt ⟨"%25"⟩;dropfelt ⟨"%11"⟩;dropfelt ⟨"%26"⟩;dropfelt ⟨"%10"⟩;Code.part6;dropfelt ⟨"%27"⟩;dropfelt ⟨"%30"⟩;Code.part7;dropfelt ⟨"%2"⟩;dropfelt ⟨"%3"⟩;dropfelt ⟨"%33"⟩;dropfelt ⟨"%34"⟩;dropfelt ⟨"%35"⟩;dropfelt ⟨"%36"⟩;Code.part8;dropfelt ⟨"%31"⟩;dropfelt ⟨"%37"⟩;dropfelt ⟨"%32"⟩;dropfelt ⟨"%38"⟩;dropfelt ⟨"%39"⟩;Code.part9;dropfelt ⟨"%40"⟩;dropfelt ⟨"%29"⟩;dropfelt ⟨"%41"⟩;dropfelt ⟨"%9"⟩;Code.part10;dropfelt ⟨"%42"⟩;dropfelt ⟨"%45"⟩;Code.part11;dropfelt ⟨"%4"⟩;dropfelt ⟨"%1"⟩;dropfelt ⟨"%48"⟩;dropfelt ⟨"%49"⟩;dropfelt ⟨"%47"⟩;dropfelt ⟨"%50"⟩;Code.part12;dropfelt ⟨"%51"⟩;dropfelt ⟨"%52"⟩;dropfelt ⟨"%53"⟩;Code.part13;dropfelt ⟨"%46"⟩;dropfelt ⟨"%54"⟩;dropfelt ⟨"%55"⟩;dropfelt ⟨"%44"⟩;Code.part14;dropfelt ⟨"%0"⟩;dropfelt ⟨"%56"⟩;dropfelt ⟨"%8"⟩;dropfelt ⟨"%57"⟩;dropfelt ⟨"%60"⟩;Code.part15;dropfelt ⟨"%61"⟩;dropfelt ⟨"%59"⟩;dropfelt ⟨"%62"⟩;dropfelt ⟨"%7"⟩;Code.part16;dropfelt ⟨"%6"⟩;dropfelt ⟨"%28"⟩;dropfelt ⟨"%43"⟩;dropfelt ⟨"%58"⟩;dropfelt ⟨"%63"⟩;dropfelt ⟨"%64"⟩) = prog
+  unfold Code.part0
+  MLIR
+  rewrite [←eq]
+  rewrite [MLIR.run_seq_def,MLIR.run_dropfelt]
+  unfold part0_state_update part0_drops part0_state
+  rfl
+
+lemma part0_cumulative_wp {x0 x1 x2 x3 y0 y1 y2 y3 y4 y5 y6 y7 y8 y9 y10 y11 y12 y13 y14 y15 y16 y17: Felt}:
+  Code.run (start_state [x0,x1,x2,x3] ([y0,y1,y2,y3,y4,y5,y6,y7,y8,y9,y10,y11,y12,y13,y14,y15,y16,y17])) ↔
+  Code.getReturn
+      (part0_state_update
+        {
+          buffers :=
+            Map.fromList
+              [({ name := "in" }, [[some x0, some x1, some x2, some x3]]),
+                ({ name := "data" },
+                  [[some y0, some y1, some y2, some y3, some y4, some y5, some y6, some y7, some y8, some y9, some y10,
+                      some y11, some y12, some y13, some y14, some y15, some y16, some y17]])],
+          bufferWidths := Map.fromList [({ name := "in" }, 4), ({ name := "data" }, 18)], constraints := [], cycle := 0,
+          felts := Map.empty, isFailed := false, props := Map.empty, vars := [{ name := "in" }, { name := "data" }] })  := by
+    unfold Code.run start_state
+    rewrite [Code.optimised_behaviour_full]
+    unfold MLIR.runProgram
+    rewrite [←Code.parts_combine]
+    unfold Code.parts_combined
+    rewrite [←Code.getReturn_ignores_drops]
+    rewrite [←Code.behaviour_with_drops]
+    rewrite [part0_wp]
+    rfl
 
 end Risc0.ComputeDecode.Constraints.WP
