Risc0/Gadgets/ComputeDecode/Constraints/WeakestPresPart2.lean
@@ -8,32 +8,49 @@ namespace Risc0.ComputeDecode.Constraints.WP
 open MLIRNotation
 
 -- The state obtained by running Code.part2 on st
-def part2_state (st: State) : State := 
-  
-        ((((st["%8"] ←ₛ getImpl st { name := "in" } 0 1)["%9"] ←ₛ getImpl st { name := "in" } 0 2)["%10"] ←ₛ
-            getImpl st { name := "in" } 0 3)["%11"] ←ₛ
-          getImpl st { name := "data" } 0
-            13) 
+def part2_state (st: State) : State :=
+  sorry
 
--- Run the whole program by using part2_state rather than Code.part2
+def part2_drops (st: State) : State :=
+  State.dropFelts (State.dropFelts (State.dropFelts (State.dropFelts (State.dropFelts (st) ⟨"%14"⟩) ⟨"%16"⟩) ⟨"%17"⟩) ⟨"%18"⟩) ⟨"%19"⟩
+
+-- Run the program from part2 onwards by using part2_state rather than Code.part2
 def part2_state_update (st: State): State :=
-  Γ (part2_state st) ⟦Code.part3; Code.part4; Code.part5; Code.part6; Code.part7; Code.part8; Code.part9; Code.part10; Code.part11; Code.part12; Code.part13; Code.part14; Code.part15; Code.part16⟧
+  Γ (part2_drops (part2_state st)) ⟦Code.part3;dropfelt ⟨"%20"⟩;dropfelt ⟨"%12"⟩;Code.part4;dropfelt ⟨"%21"⟩;dropfelt ⟨"%5"⟩;dropfelt ⟨"%22"⟩;dropfelt ⟨"%23"⟩;dropfelt ⟨"%24"⟩;Code.part5;dropfelt ⟨"%25"⟩;dropfelt ⟨"%11"⟩;dropfelt ⟨"%26"⟩;dropfelt ⟨"%10"⟩;Code.part6;dropfelt ⟨"%27"⟩;dropfelt ⟨"%30"⟩;Code.part7;dropfelt ⟨"%2"⟩;dropfelt ⟨"%3"⟩;dropfelt ⟨"%33"⟩;dropfelt ⟨"%34"⟩;dropfelt ⟨"%35"⟩;dropfelt ⟨"%36"⟩;Code.part8;dropfelt ⟨"%31"⟩;dropfelt ⟨"%37"⟩;dropfelt ⟨"%32"⟩;dropfelt ⟨"%38"⟩;dropfelt ⟨"%39"⟩;Code.part9;dropfelt ⟨"%40"⟩;dropfelt ⟨"%29"⟩;dropfelt ⟨"%41"⟩;dropfelt ⟨"%9"⟩;Code.part10;dropfelt ⟨"%42"⟩;dropfelt ⟨"%45"⟩;Code.part11;dropfelt ⟨"%4"⟩;dropfelt ⟨"%1"⟩;dropfelt ⟨"%48"⟩;dropfelt ⟨"%49"⟩;dropfelt ⟨"%47"⟩;dropfelt ⟨"%50"⟩;Code.part12;dropfelt ⟨"%51"⟩;dropfelt ⟨"%52"⟩;dropfelt ⟨"%53"⟩;Code.part13;dropfelt ⟨"%46"⟩;dropfelt ⟨"%54"⟩;dropfelt ⟨"%55"⟩;dropfelt ⟨"%44"⟩;Code.part14;dropfelt ⟨"%0"⟩;dropfelt ⟨"%56"⟩;dropfelt ⟨"%8"⟩;dropfelt ⟨"%57"⟩;dropfelt ⟨"%60"⟩;Code.part15;dropfelt ⟨"%61"⟩;dropfelt ⟨"%59"⟩;dropfelt ⟨"%62"⟩;dropfelt ⟨"%7"⟩;Code.part16;dropfelt ⟨"%6"⟩;dropfelt ⟨"%28"⟩;dropfelt ⟨"%43"⟩;dropfelt ⟨"%58"⟩;dropfelt ⟨"%63"⟩;dropfelt ⟨"%64"⟩⟧
 
 -- Prove that substituting part2_state for Code.part2 produces the same result
 lemma part2_wp {st : State} :
-  Code.getReturn (MLIR.runProgram (Code.part2; Code.part3; Code.part4; Code.part5; Code.part6; Code.part7; Code.part8; Code.part9; Code.part10; Code.part11; Code.part12; Code.part13; Code.part14; Code.part15; Code.part16) st) ↔
+  Code.getReturn (MLIR.runProgram (Code.part2;dropfelt ⟨"%14"⟩;dropfelt ⟨"%16"⟩;dropfelt ⟨"%17"⟩;dropfelt ⟨"%18"⟩;dropfelt ⟨"%19"⟩;Code.part3;dropfelt ⟨"%20"⟩;dropfelt ⟨"%12"⟩;Code.part4;dropfelt ⟨"%21"⟩;dropfelt ⟨"%5"⟩;dropfelt ⟨"%22"⟩;dropfelt ⟨"%23"⟩;dropfelt ⟨"%24"⟩;Code.part5;dropfelt ⟨"%25"⟩;dropfelt ⟨"%11"⟩;dropfelt ⟨"%26"⟩;dropfelt ⟨"%10"⟩;Code.part6;dropfelt ⟨"%27"⟩;dropfelt ⟨"%30"⟩;Code.part7;dropfelt ⟨"%2"⟩;dropfelt ⟨"%3"⟩;dropfelt ⟨"%33"⟩;dropfelt ⟨"%34"⟩;dropfelt ⟨"%35"⟩;dropfelt ⟨"%36"⟩;Code.part8;dropfelt ⟨"%31"⟩;dropfelt ⟨"%37"⟩;dropfelt ⟨"%32"⟩;dropfelt ⟨"%38"⟩;dropfelt ⟨"%39"⟩;Code.part9;dropfelt ⟨"%40"⟩;dropfelt ⟨"%29"⟩;dropfelt ⟨"%41"⟩;dropfelt ⟨"%9"⟩;Code.part10;dropfelt ⟨"%42"⟩;dropfelt ⟨"%45"⟩;Code.part11;dropfelt ⟨"%4"⟩;dropfelt ⟨"%1"⟩;dropfelt ⟨"%48"⟩;dropfelt ⟨"%49"⟩;dropfelt ⟨"%47"⟩;dropfelt ⟨"%50"⟩;Code.part12;dropfelt ⟨"%51"⟩;dropfelt ⟨"%52"⟩;dropfelt ⟨"%53"⟩;Code.part13;dropfelt ⟨"%46"⟩;dropfelt ⟨"%54"⟩;dropfelt ⟨"%55"⟩;dropfelt ⟨"%44"⟩;Code.part14;dropfelt ⟨"%0"⟩;dropfelt ⟨"%56"⟩;dropfelt ⟨"%8"⟩;dropfelt ⟨"%57"⟩;dropfelt ⟨"%60"⟩;Code.part15;dropfelt ⟨"%61"⟩;dropfelt ⟨"%59"⟩;dropfelt ⟨"%62"⟩;dropfelt ⟨"%7"⟩;Code.part16;dropfelt ⟨"%6"⟩;dropfelt ⟨"%28"⟩;dropfelt ⟨"%43"⟩;dropfelt ⟨"%58"⟩;dropfelt ⟨"%63"⟩;dropfelt ⟨"%64"⟩) st) ↔
   Code.getReturn (part2_state_update st) := by
   unfold MLIR.runProgram; simp only
-  generalize eq : (Code.part3; Code.part4; Code.part5; Code.part6; Code.part7; Code.part8; Code.part9; Code.part10; Code.part11; Code.part12; Code.part13; Code.part14; Code.part15; Code.part16) = prog
+  generalize eq : (dropfelt ⟨"%14"⟩;dropfelt ⟨"%16"⟩;dropfelt ⟨"%17"⟩;dropfelt ⟨"%18"⟩;dropfelt ⟨"%19"⟩;Code.part3;dropfelt ⟨"%20"⟩;dropfelt ⟨"%12"⟩;Code.part4;dropfelt ⟨"%21"⟩;dropfelt ⟨"%5"⟩;dropfelt ⟨"%22"⟩;dropfelt ⟨"%23"⟩;dropfelt ⟨"%24"⟩;Code.part5;dropfelt ⟨"%25"⟩;dropfelt ⟨"%11"⟩;dropfelt ⟨"%26"⟩;dropfelt ⟨"%10"⟩;Code.part6;dropfelt ⟨"%27"⟩;dropfelt ⟨"%30"⟩;Code.part7;dropfelt ⟨"%2"⟩;dropfelt ⟨"%3"⟩;dropfelt ⟨"%33"⟩;dropfelt ⟨"%34"⟩;dropfelt ⟨"%35"⟩;dropfelt ⟨"%36"⟩;Code.part8;dropfelt ⟨"%31"⟩;dropfelt ⟨"%37"⟩;dropfelt ⟨"%32"⟩;dropfelt ⟨"%38"⟩;dropfelt ⟨"%39"⟩;Code.part9;dropfelt ⟨"%40"⟩;dropfelt ⟨"%29"⟩;dropfelt ⟨"%41"⟩;dropfelt ⟨"%9"⟩;Code.part10;dropfelt ⟨"%42"⟩;dropfelt ⟨"%45"⟩;Code.part11;dropfelt ⟨"%4"⟩;dropfelt ⟨"%1"⟩;dropfelt ⟨"%48"⟩;dropfelt ⟨"%49"⟩;dropfelt ⟨"%47"⟩;dropfelt ⟨"%50"⟩;Code.part12;dropfelt ⟨"%51"⟩;dropfelt ⟨"%52"⟩;dropfelt ⟨"%53"⟩;Code.part13;dropfelt ⟨"%46"⟩;dropfelt ⟨"%54"⟩;dropfelt ⟨"%55"⟩;dropfelt ⟨"%44"⟩;Code.part14;dropfelt ⟨"%0"⟩;dropfelt ⟨"%56"⟩;dropfelt ⟨"%8"⟩;dropfelt ⟨"%57"⟩;dropfelt ⟨"%60"⟩;Code.part15;dropfelt ⟨"%61"⟩;dropfelt ⟨"%59"⟩;dropfelt ⟨"%62"⟩;dropfelt ⟨"%7"⟩;Code.part16;dropfelt ⟨"%6"⟩;dropfelt ⟨"%28"⟩;dropfelt ⟨"%43"⟩;dropfelt ⟨"%58"⟩;dropfelt ⟨"%63"⟩;dropfelt ⟨"%64"⟩) = prog
   unfold Code.part2
   MLIR
-  unfold part2_state_update part2_state
-  rewrite [←eq]
-  rfl
 
 lemma part2_updates_opaque {st : State} : 
   Code.getReturn (part1_state_update st) ↔
-  Code.getReturn (part2_state_update (part1_state st)) := by
+  Code.getReturn (part2_state_update (part1_drops (part1_state st))) := by
   simp [part1_state_update, part2_wp]
+
+lemma part2_cumulative_wp {x0 x1 x2 x3 y0 y1 y2 y3 y4 y5 y6 y7 y8 y9 y10 y11 y12 y13 y14 y15 y16 y17: Felt} :
+  Code.run (start_state [x0,x1,x2,x3] ([y0,y1,y2,y3,y4,y5,y6,y7,y8,y9,y10,y11,y12,y13,y14,y15,y16,y17])) ↔
+  sorry := by
+    rewrite [part1_cumulative_wp]
+    rewrite [part2_updates_opaque]
+    unfold part1_state
+    MLIR_states_updates
+    -- 0 withEqZeros
+    -- rewrite [withEqZero_def]
+    -- MLIR_states_updates
+    unfold part1_drops
+    -- 1 drop
+    simp only [State.drop_update_swap, State.drop_update_same]
+    rewrite [State.dropFelts]
+    simp only [State.dropFelts_buffers, State.dropFelts_bufferWidths, State.dropFelts_constraints, State.dropFelts_cycle, State.dropFelts_felts, State.dropFelts_isFailed, State.dropFelts_props, State.dropFelts_vars]
+    simp only [Map.drop_base, ne_eq, Map.update_drop_swap, Map.update_drop]
+    -- 0 sets
+    -- rewrite [Map.drop_of_updates]
+    -- simp only [Map.drop_base, ne_eq, Map.update_drop_swap, Map.update_drop]
+    rfl
 
 end Risc0.ComputeDecode.Constraints.WP
