Risc0/Optimisation.lean
@@ -17,221 +17,214 @@ lemma updateFelts_neq_comm {st : State} {name name' : FeltVar} {v v' : Felt} (h 
   rw [Map.update_neq_comm]
   exact h
 
+lemma opt_swap (h: Γ (Γ st ⟦p₁⟧) ⟦p₂⟧ = Γ (Γ st ⟦p₂⟧) ⟦p₁⟧) :
+  Γ st ⟦p₁; p₂; p₃⟧ = Γ ( Γ st ⟦p₂⟧) ⟦p₁; p₃⟧ := by
+    simp [MLIR.run_seq_def, h]
+
+lemma opt_swap_nondet_single (h: Γ (Γ st ⟦p₁⟧) ⟦p₂⟧ = Γ (Γ st ⟦p₂⟧) ⟦p₁⟧) :
+  Γ st ⟦p₁; nondet p₂; p₃⟧ = Γ ( Γ st ⟦p₂⟧) ⟦p₁; p₃⟧ := by
+    simp [MLIR.run_seq_def, MLIR.run_nondet, h]
+
+lemma opt_swap_nondet_seq (h: Γ (Γ st ⟦p₁⟧) ⟦p₂⟧ = Γ (Γ st ⟦p₂⟧) ⟦p₁⟧) :
+  Γ st ⟦p₁; nondet (p₂; p₃); p₄⟧ = Γ ( Γ st ⟦p₂⟧) ⟦p₁; nondet p₃; p₄⟧ := by
+    simp [MLIR.run_seq_def, MLIR.run_nondet, h]
+
+lemma opt_swap_ddd (h: Γ (Γ st ⟦p₁⟧) ⟦p₂⟧ = Γ (Γ st ⟦p₂⟧) ⟦p₁⟧) :
+  Γ st ⟦p₁; p₂; p₃⟧ = Γ (Γ st ⟦p₂⟧) ⟦p₁; p₃⟧ := by
+    simp [MLIR.run_seq_def, h]
+
+lemma opt_swap_ndd (h: Γ (Γ st ⟦p₁⟧) ⟦p₂⟧ = Γ (Γ st ⟦p₂⟧) ⟦p₁⟧) :
+  Γ st ⟦nondet p₁; p₂; p₃⟧ = Γ (Γ st ⟦p₂⟧) ⟦nondet p₁; p₃⟧ := by
+    simp [MLIR.run_seq_def, MLIR.run_nondet, h]
+
+lemma opt_swap_dnd (h: Γ (Γ st ⟦p₁⟧) ⟦p₂⟧ = Γ (Γ st ⟦p₂⟧) ⟦p₁⟧) :
+  Γ st ⟦p₁; nondet p₂; p₃⟧ = Γ (Γ st ⟦p₂⟧) ⟦p₁; p₃⟧ := by
+    simp [MLIR.run_seq_def, MLIR.run_nondet, h]
+
+lemma opt_swap_nnd (h: Γ (Γ st ⟦p₁⟧) ⟦p₂⟧ = Γ (Γ st ⟦p₂⟧) ⟦p₁⟧) :
+  Γ st ⟦nondet (p₁; p₂); p₃⟧ = Γ (Γ st ⟦p₂⟧) ⟦nondet p₁; p₃⟧ := by
+    simp [MLIR.run_seq_def, MLIR.run_nondet, h]
+
+lemma opt_swap_ddn (h: Γ (Γ st ⟦p₁⟧) ⟦p₂⟧ = Γ (Γ st ⟦p₂⟧) ⟦p₁⟧) :
+  Γ st ⟦p₁; p₂; nondet p₃⟧ = Γ (Γ st ⟦p₂⟧) ⟦p₁; nondet p₃⟧ := by
+    simp [MLIR.run_seq_def, h]
+
+lemma opt_swap_ndn (h: Γ (Γ st ⟦p₁⟧) ⟦p₂⟧ = Γ (Γ st ⟦p₂⟧) ⟦p₁⟧) :
+  Γ st ⟦nondet p₁; p₂; nondet p₃⟧ = Γ (Γ st ⟦p₂⟧) ⟦nondet (p₁; p₃)⟧ := by
+    simp [MLIR.run_seq_def, MLIR.run_nondet, h]
+
+lemma opt_swap_dnn (h: Γ (Γ st ⟦p₁⟧) ⟦p₂⟧ = Γ (Γ st ⟦p₂⟧) ⟦p₁⟧) :
+  Γ st ⟦p₁; nondet (p₂; p₃)⟧ = Γ (Γ st ⟦p₂⟧) ⟦p₁; nondet p₃⟧ := by
+    simp [MLIR.run_seq_def, MLIR.run_nondet, h]
+
+lemma opt_swap_nnn (h: Γ (Γ st ⟦p₁⟧) ⟦p₂⟧ = Γ (Γ st ⟦p₂⟧) ⟦p₁⟧) :
+  Γ st ⟦nondet (p₁; p₂; p₃)⟧ = Γ (Γ st ⟦p₂⟧) ⟦nondet (p₁; p₃)⟧ := by
+    simp [MLIR.run_seq_def, MLIR.run_nondet, h]
+
 section add
+  lemma add_past_const (h: a ≠ b) (h': ⟨b⟩ ≠ c) (h'': ⟨b⟩ ≠ d):
+    Γ (Γ st ⟦@MLIR.Assign α a (Op.Add c d)⟧) ⟦@MLIR.Assign β b (Op.Const x)⟧ =
+    Γ (Γ st ⟦@MLIR.Assign β b (Op.Const x)⟧) ⟦@MLIR.Assign α a (Op.Add c d)⟧ := by
+      simp [MLIR.run_ass_def]
+      rewrite [updateFelts_neq_comm] <;> aesop
+
   lemma add_past_drop (h : name ≠ name') (h₁ : ⟨name'⟩ ≠ lhs) (h₂ : ⟨name'⟩ ≠ rhs) :
-    Γ st ⟦name ←ₐ .Add lhs rhs; @MLIR.DropFelt α ⟨name'⟩⟧ =
-    Γ st ⟦@MLIR.DropFelt α ⟨name'⟩; name ←ₐ .Add lhs rhs⟧ := by
-      MLIR
-      simp [State.drop_update_swap, h]
-      unfold State.dropFelts Map.drop State.updateFelts
+    Γ (Γ st ⟦@MLIR.Assign α name (Op.Add lhs rhs)⟧) ⟦@MLIR.DropFelt β ⟨name'⟩⟧ =
+    Γ (Γ st ⟦@MLIR.DropFelt β ⟨name'⟩⟧) ⟦@MLIR.Assign α name (Op.Add lhs rhs)⟧ := by
+      simp [MLIR.run_ass_def, MLIR.run_dropfelt]
       aesop
 end add
 
+section andeqz
+  lemma andEqz_past_const (h: ⟨b⟩ ≠ d):
+    Γ (Γ st ⟦@MLIR.Assign α a (Op.AndEqz c d)⟧) ⟦@MLIR.Assign β b (Op.Const x)⟧ =
+    Γ (Γ st ⟦@MLIR.Assign β b (Op.Const x)⟧) ⟦@MLIR.Assign α a (Op.AndEqz c d)⟧ := by
+      simp [MLIR.run_ass_def, State.updateFelts, State.updateProps, *, Map.update]
+      aesop
+  
+  lemma andEqz_past_drop (h : ⟨x⟩ ≠ y) (h₁ : rhs ≠ y) :
+    Γ (Γ st ⟦@MLIR.Assign β x (Op.AndEqz lhs rhs)⟧) ⟦@MLIR.DropFelt α y⟧ =
+    Γ (Γ st ⟦@MLIR.DropFelt α y⟧) ⟦@MLIR.Assign β x (Op.AndEqz lhs rhs)⟧ := by
+      simp [
+        MLIR.run_ass_def, MLIR.run_dropfelt, State.updateFelts, State.updateProps, Map.update,
+        State.dropFelts, Map.drop
+      ]
+      aesop
+end andeqz
+
 section bitand
-  lemma bitand_past_drop (h : name ≠ name') (h₁ : ⟨name'⟩ ≠ lhs) (h₂ : ⟨name'⟩ ≠ rhs):
-    Γ st ⟦name ←ₐ .BitAnd lhs rhs; @MLIR.DropFelt α ⟨name'⟩⟧ =
-    Γ st ⟦@MLIR.DropFelt α ⟨name'⟩; name ←ₐ .BitAnd lhs rhs⟧ := by
-      MLIR
-      simp [State.drop_update_swap, h, feltBitAnd, State.get_dropFelts_of_ne h₁]
+  lemma bitAnd_past_const (h: a ≠ b) (h': ⟨b⟩ ≠ c) (h'': ⟨b⟩ ≠ d):
+    Γ (Γ st ⟦@MLIR.Assign α a (Op.BitAnd c d)⟧) ⟦@MLIR.Assign β b (Op.Const x)⟧ =
+    Γ (Γ st ⟦@MLIR.Assign β b (Op.Const x)⟧) ⟦@MLIR.Assign α a (Op.BitAnd c d)⟧ := by
+      simp [MLIR.run_ass_def]
+      rewrite [updateFelts_neq_comm] <;> aesop
+
+  lemma bitAnd_past_drop (h : name ≠ name') (h₁ : ⟨name'⟩ ≠ lhs) (h₂ : ⟨name'⟩ ≠ rhs):
+    Γ (Γ st ⟦@MLIR.Assign α name (Op.BitAnd lhs rhs)⟧) ⟦@MLIR.DropFelt β ⟨name'⟩⟧ =
+    Γ (Γ st ⟦@MLIR.DropFelt β ⟨name'⟩⟧) ⟦@MLIR.Assign α name (Op.BitAnd lhs rhs)⟧ := by
+      simp [MLIR.run_ass_def, MLIR.run_dropfelt]
       aesop
 end bitand
 
 section const
   lemma const_past_add (h: a ≠ b) (h': ⟨a⟩ ≠ c) (h'': ⟨a⟩ ≠ d):
-    State.buffers (Γ st ⟦a ←ₐ C x; b ←ₐ Op.Add c d; rest⟧) =
-    State.buffers (Γ st ⟦b ←ₐ Op.Add c d; a ←ₐ C x; rest⟧) := by
-      MLIR
-      rewrite [updateFelts_neq_comm] <;> simp [*]
+    Γ (Γ st ⟦@MLIR.Assign α a (Op.Const x)⟧) ⟦@MLIR.Assign β b (Op.Add c d)⟧ =
+    Γ (Γ st ⟦@MLIR.Assign β b (Op.Add c d)⟧) ⟦@MLIR.Assign α a (Op.Const x)⟧ := by
+      rw [add_past_const] <;> aesop
+  
+  lemma const_past_andEqz (h: ⟨b⟩ ≠ d):
+    Γ (Γ st ⟦@MLIR.Assign β b (Op.Const x)⟧) ⟦@MLIR.Assign α a (Op.AndEqz c d)⟧ =
+    Γ (Γ st ⟦@MLIR.Assign α a (Op.AndEqz c d)⟧) ⟦@MLIR.Assign β b (Op.Const x)⟧ := by
+      rw [andEqz_past_const]
+      aesop
 
   lemma const_past_bitAnd (h: a ≠ b) (h': ⟨a⟩ ≠ c) (h'': ⟨a⟩ ≠ d):
-    State.buffers (Γ st ⟦a ←ₐ C x; b ←ₐ Op.BitAnd c d; rest⟧) =
-    State.buffers (Γ st ⟦b ←ₐ Op.BitAnd c d; a ←ₐ C x; rest⟧) := by
-      MLIR
-      rewrite [updateFelts_neq_comm] <;> simp [*]
-
-  lemma const_past_bitAnd_nondet (h: a ≠ b) (h': ⟨a⟩ ≠ c) (h'': ⟨a⟩ ≠ d):
-    State.buffers (Γ st ⟦a ←ₐ C x; nondet(b ←ₐ Op.BitAnd c d; s₁); s₂⟧) =
-    State.buffers (Γ st ⟦nondet (b ←ₐ Op.BitAnd c d); a ←ₐ C x; nondet s₁; s₂⟧) := by
-      MLIR
-      rewrite [updateFelts_neq_comm] <;> simp [*]
-
-  lemma const_past_bitAnd_nondet_single (h: a ≠ b) (h': ⟨a⟩ ≠ c) (h'': ⟨a⟩ ≠ d):
-    State.buffers (Γ st ⟦a ←ₐ C x; nondet(b ←ₐ Op.BitAnd c d); s₂⟧) =
-    State.buffers (Γ st ⟦nondet (b ←ₐ Op.BitAnd c d); a ←ₐ C x; s₂⟧) := by
-      MLIR
-      rewrite [updateFelts_neq_comm] <;> simp [*]
+    Γ (Γ st ⟦@MLIR.Assign α a (Op.Const x)⟧) ⟦@MLIR.Assign β b (Op.BitAnd c d)⟧ =
+    Γ (Γ st ⟦@MLIR.Assign β b (Op.BitAnd c d)⟧) ⟦@MLIR.Assign α a (Op.Const x)⟧ := by
+      rw [bitAnd_past_const] <;> aesop
 
   lemma const_past_const (h: x ≠ y):
-    State.buffers (Γ st ⟦x ←ₐ C c₁; y ←ₐ C c₂; rest⟧) =
-    State.buffers (Γ st ⟦y ←ₐ C c₂; x ←ₐ C c₁; rest⟧) := by
-      simp [MLIR.run_seq_def, MLIR.run_ass_def, Op.eval_const]
-      rewrite [updateFelts_neq_comm] <;> simp [*]
+    Γ (Γ st ⟦@MLIR.Assign α x (Op.Const c₁)⟧) ⟦@MLIR.Assign β y (Op.Const c₂)⟧ =
+    Γ (Γ st ⟦@MLIR.Assign β y (Op.Const c₂)⟧) ⟦@MLIR.Assign α x (Op.Const c₁)⟧ := by
+      simp [MLIR.run_ass_def]
+      rewrite [updateFelts_neq_comm] <;> aesop
 
   lemma const_past_drop (h : name ≠ name') :
-    Γ st ⟦name ←ₐ C x; @MLIR.DropFelt α ⟨name'⟩⟧ =
-    Γ st ⟦@MLIR.DropFelt α ⟨name'⟩; name ←ₐ C x⟧ := by
-      MLIR
-      simp [State.drop_update_swap, h]
+    Γ (Γ st ⟦@MLIR.Assign α name (Op.Const x)⟧) ⟦@MLIR.DropFelt β ⟨name'⟩⟧ =
+    Γ (Γ st ⟦@MLIR.DropFelt β ⟨name'⟩⟧) ⟦@MLIR.Assign α name (Op.Const x)⟧ := by
+      simp [MLIR.run_ass_def, MLIR.run_dropfelt]
+      aesop
 
   lemma const_past_get (h: x ≠ y):
-    State.buffers (Γ st ⟦x ←ₐ C c₁; y ←ₐ .Get buf back offset; rest⟧) =
-    State.buffers (Γ st ⟦y ←ₐ .Get buf back offset; x ←ₐ C c₁; rest⟧) := by
-      simp [MLIR.run_seq_def, MLIR.run_ass_def, Op.eval_const]
+    Γ (Γ st ⟦@MLIR.Assign α x (Op.Const c₁)⟧) ⟦@MLIR.Assign β y (Op.Get buf back offset)⟧ =
+    Γ (Γ st ⟦@MLIR.Assign β y (Op.Get buf back offset)⟧) ⟦@MLIR.Assign α x (Op.Const c₁)⟧ := by
+      simp [MLIR.run_ass_def]
       aesop
       rewrite [updateFelts_neq_comm] <;> simp [*]
-
-  lemma const_past_nondet :
-    State.buffers (Γ st ⟦x ←ₐ C c₁; nondet p; rest⟧) =
-    State.buffers (Γ st ⟦nondet (x ←ₐ C c₁; p); rest⟧) := by
-      simp [MLIR.run_seq_def, MLIR.run_nondet]
-      rfl
 
   lemma const_past_mul (h: a ≠ b) (h': ⟨a⟩ ≠ c) (h'': ⟨a⟩ ≠ d):
-    State.buffers (Γ st ⟦a ←ₐ C x; b ←ₐ Op.Mul c d; rest⟧) =
-    State.buffers (Γ st ⟦b ←ₐ Op.Mul c d; a ←ₐ C x; rest⟧) := by
-      MLIR
+    Γ (Γ st ⟦@MLIR.Assign α a (Op.Const x)⟧) ⟦@MLIR.Assign β b (Op.Mul c d)⟧ =
+    Γ (Γ st ⟦@MLIR.Assign β b (Op.Mul c d)⟧) ⟦@MLIR.Assign α a (Op.Const x)⟧ := by
+      simp [MLIR.run_ass_def]
       rewrite [updateFelts_neq_comm] <;> simp [*]
 
-  lemma const_past_mul_nondet (h: a ≠ b) (h': ⟨a⟩ ≠ c) (h'': ⟨a⟩ ≠ d):
-    State.buffers (Γ st ⟦a ←ₐ C x; nondet(b ←ₐ Op.Mul c d; s₁); s₂⟧) =
-    State.buffers (Γ st ⟦nondet (b ←ₐ Op.Mul c d); a ←ₐ C x; nondet s₁; s₂⟧) := by
-      MLIR
-      rewrite [updateFelts_neq_comm] <;> simp [*]
-
-  lemma const_past_mul_nondet_single (h: a ≠ b) (h': ⟨a⟩ ≠ c) (h'': ⟨a⟩ ≠ d):
-    State.buffers (Γ st ⟦a ←ₐ C x; nondet(b ←ₐ Op.Mul c d); s₂⟧) =
-    State.buffers (Γ st ⟦nondet (b ←ₐ Op.Mul c d); a ←ₐ C x; s₂⟧) := by
-      MLIR
-      rewrite [updateFelts_neq_comm] <;> simp [*]
-
-  lemma const_past_set_nondet (h: ⟨a⟩ ≠ d) :
-    State.buffers (Γ st ⟦a ←ₐ C x; nondet(b[c] ←ᵢ d; s₁); s₂⟧) =
-    State.buffers (Γ st ⟦nondet(b[c] ←ᵢ d); a ←ₐ C x; nondet s₁; s₂⟧) := by
-      MLIR
-      simp [State.set!, State.setBufferElementImpl]
+  lemma const_past_set (h: ⟨a⟩ ≠ b) :
+    Γ (Γ st ⟦@MLIR.Assign α a (Op.Const x)⟧) ⟦@MLIR.Set buf offset b⟧ =
+    Γ (Γ st ⟦@MLIR.Set buf offset b⟧) ⟦@MLIR.Assign α a (Op.Const x)⟧ := by
+      simp [MLIR.run_ass_def, MLIR.run_set_def, State.set!, State.setBufferElementImpl]
       aesop
 
-  lemma const_past_set_nondet_single (h: ⟨a⟩ ≠ d) :
-    State.buffers (Γ st ⟦a ←ₐ C x; nondet(b[c] ←ᵢ d); s₂⟧) =
-    State.buffers (Γ st ⟦nondet(b[c] ←ᵢ d); a ←ₐ C x; s₂⟧) := by
-      MLIR
-      simp [State.set!, State.setBufferElementImpl]
+  lemma const_past_sub (h: a ≠ b) (h': ⟨a⟩ ≠ c) (h'': ⟨a⟩ ≠ d):
+    Γ (Γ st ⟦@MLIR.Assign α a (Op.Const x)⟧) ⟦@MLIR.Assign β b (Op.Sub c d)⟧ =
+    Γ (Γ st ⟦@MLIR.Assign β b (Op.Sub c d)⟧) ⟦@MLIR.Assign α a (Op.Const x)⟧ := by
+      simp [MLIR.run_ass_def]
+      rewrite [updateFelts_neq_comm] <;> aesop
+  
+  lemma const_past_true (h: a ≠ b) :
+    Γ (Γ st ⟦@MLIR.Assign α a (Op.Const x)⟧) ⟦@MLIR.Assign β b (Op.True)⟧ =
+    Γ (Γ st ⟦@MLIR.Assign β b (Op.True)⟧) ⟦@MLIR.Assign α a (Op.Const x)⟧ := by
+      simp [MLIR.run_ass_def]
       aesop
+
 end const
 
 section drop
 
   lemma drop_past_add (h : ⟨x⟩ ≠ y) (h₁ : lhs ≠ y) (h₂ : rhs ≠ y) :
-    (Γ st ⟦@MLIR.DropFelt α y; x ←ₐ .Add lhs rhs⟧) =
-    (Γ st ⟦x ←ₐ .Add lhs rhs; @MLIR.DropFelt α y⟧) := by
-      MLIR
-      simp [State.drop_update_swap, h]
-      unfold State.dropFelts Map.drop State.updateFelts
-      aesop
-  lemma drop_past_add_single (h : ⟨x⟩ ≠ y) (h₁ : lhs ≠ y) (h₂ : rhs ≠ y) :
-    State.buffers (Γ st ⟦@MLIR.DropFelt α y; x ←ₐ .Add lhs rhs⟧) =
-    State.buffers (Γ st ⟦x ←ₐ .Add lhs rhs; @MLIR.DropFelt α y⟧) := by
-      MLIR
-      simp [State.drop_update_swap, h]
+    Γ (Γ st ⟦@MLIR.DropFelt α y⟧) ⟦@MLIR.Assign β x (Op.Add lhs rhs)⟧ =
+    Γ (Γ st ⟦@MLIR.Assign β x (Op.Add lhs rhs)⟧) ⟦@MLIR.DropFelt α y⟧ := by
+      rw [add_past_drop] <;> aesop
 
-  lemma drop_past_bitAnd_nondet (h : ⟨x⟩ ≠ y) (h₁ : lhs ≠ y) (h₂ : rhs ≠ y):
-    Γ st ⟦dropfelt y; nondet (x ←ₐ .BitAnd lhs rhs)⟧ =
-    Γ st ⟦nondet(x ←ₐ .BitAnd lhs rhs); dropfelt y⟧ := by
-      sorry
-      -- MLIR
-      -- simp [State.drop_update_swap, h, feltBitAnd, State.get_dropFelts_of_ne h₁.symm]
-      -- aesop
+  lemma drop_past_andEqz (h : ⟨x⟩ ≠ y) (h₁ : rhs ≠ y) :
+    Γ (Γ st ⟦@MLIR.DropFelt α y⟧) ⟦@MLIR.Assign β x (Op.AndEqz lhs rhs)⟧ =
+    Γ (Γ st ⟦@MLIR.Assign β x (Op.AndEqz lhs rhs)⟧) ⟦@MLIR.DropFelt α y⟧ := by
+      rw [andEqz_past_drop] <;> aesop
+
+  lemma drop_past_bitAnd (h : ⟨x⟩ ≠ y) (h₁ : lhs ≠ y) (h₂ : rhs ≠ y):
+    Γ (Γ st ⟦@MLIR.DropFelt α y⟧) ⟦@MLIR.Assign β x (Op.BitAnd lhs rhs)⟧ =
+    Γ (Γ st ⟦@MLIR.Assign β x (Op.BitAnd lhs rhs)⟧) ⟦@MLIR.DropFelt α y⟧ := by
+      rw [bitAnd_past_drop] <;> aesop
 
   lemma drop_past_const (h : ⟨x⟩ ≠ y) :
-    Γ st ⟦@MLIR.DropFelt α y; x ←ₐ C c⟧ =
-    Γ st ⟦x ←ₐ C c; @MLIR.DropFelt α y⟧ := by
-      MLIR
-      simp [State.drop_update_swap, h]
+    Γ (Γ st ⟦@MLIR.DropFelt α y⟧) ⟦@MLIR.Assign β x (Op.Const c)⟧ =
+    Γ (Γ st ⟦@MLIR.Assign β x (Op.Const c)⟧) ⟦@MLIR.DropFelt α y⟧ := by
+      rw [const_past_drop]; aesop
 
   lemma drop_past_eqz (h : x ≠ y) :
-    (Γ st ⟦dropfelt y; @MLIR.Eqz IsNondet.NotInNondet x⟧) =
-    (Γ st ⟦@MLIR.Eqz IsNondet.NotInNondet x; dropfelt y⟧) := by
-      sorry
-
-  lemma drop_past_eqz_single (h : x ≠ y) :
-    State.buffers (Γ st ⟦dropfelt y; @MLIR.Eqz IsNondet.NotInNondet x⟧) =
-    State.buffers (Γ st ⟦@MLIR.Eqz IsNondet.NotInNondet x; dropfelt y⟧) := by
-    MLIR
-    simp [State.dropFelts, Map.drop]
+    Γ (Γ st ⟦@MLIR.DropFelt α y⟧) ⟦@MLIR.Eqz β x⟧ =
+    Γ (Γ st ⟦@MLIR.Eqz β x⟧) ⟦@MLIR.DropFelt α y⟧ := by
+      simp [MLIR.run_dropfelt, MLIR.run_eqz, withEqZero, State.dropFelts, Map.drop]
+      sorry --map[x]! issues introduced by eqz
 
   lemma drop_past_get (h: ⟨x⟩ ≠ y) :
-    (Γ st ⟦@MLIR.DropFelt α y; x ←ₐ .Get buf back offset⟧) =
-    (Γ st ⟦x ←ₐ .Get buf back offset; @MLIR.DropFelt α y⟧) := by
-      MLIR
-      generalize eq: getImpl st buf back offset = get
-      cases get with
-        | none => aesop
-        | some lit =>
-          have h_lit: ∃ k, lit = Lit.Val k := getImpl_val_of_some eq
-          aesop
+    Γ (Γ st ⟦@MLIR.DropFelt α y⟧) ⟦@MLIR.Assign β x (Op.Get buf back offset)⟧ =
+    Γ (Γ st ⟦@MLIR.Assign β x (Op.Get buf back offset)⟧) ⟦@MLIR.DropFelt α y⟧ := by
+      simp [MLIR.run_dropfelt, MLIR.run_ass_def]
+      sorry
   
-  lemma drop_past_get_single (h: ⟨x⟩ ≠ y) :
-    State.buffers (Γ st ⟦@MLIR.DropFelt α y; x ←ₐ .Get buf back offset⟧) =
-    State.buffers (Γ st ⟦x ←ₐ .Get buf back offset; @MLIR.DropFelt α y⟧) := by
-      MLIR
-      generalize eq: getImpl st buf back offset = get
-      cases get with
-        | none => aesop
-        | some lit =>
-          have h_lit: ∃ k, lit = Lit.Val k := getImpl_val_of_some eq
-          aesop
-  
-  lemma drop_past_if (h : y ≠ c) (h₁ : y ∉ st.felts) :
-    Γ st ⟦dropfelt y; guard c then prog⟧ =
-    Γ st ⟦guard c then (dropfelt y; prog)⟧ := by
-    MLIR
-    simp [getElem!, State.get_dropFelts_of_ne h]
-    aesop; aesop
-    rw [Map.not_mem_iff_none, Map.getElem_def] at h₁
-    unfold State.dropFelts Map.drop
-    congr
-    funext z
-    aesop
+  -- lemma drop_past_if (h : y ≠ x) (h₁ : Γ (Γ st ⟦@MLIR.DropFelt α y⟧) ⟦prog⟧ = Γ (Γ st ⟦prog⟧) ⟦@MLIR.DropFelt α y⟧) :
+  --   Γ (Γ st ⟦@MLIR.DropFelt α y⟧) ⟦@MLIR.If β x prog⟧ =
+  --   Γ (Γ st ⟦@MLIR.If β x prog⟧) ⟦@MLIR.DropFelt α y⟧ := by
+  --     simp [MLIR.run_dropfelt, MLIR.run_if]
+  --     simp [getElem!, State.get_dropFelts_of_ne h]
+      
+  --     -- MLIR
+  --     -- aesop; aesop
+  --     -- rw [Map.not_mem_iff_none, Map.getElem_def] at h₁
+  --     -- unfold State.dropFelts Map.drop
+  --     -- congr
+  --     -- funext z
+  --     -- aesop
 
   lemma drop_past_mul (h : ⟨x⟩ ≠ y) (h₁ : lhs ≠ y) (h₂ : rhs ≠ y) :
-    (Γ st ⟦@MLIR.DropFelt α y; x ←ₐ .Mul lhs rhs⟧) =
-    (Γ st ⟦x ←ₐ .Mul lhs rhs; @MLIR.DropFelt α y⟧) := by
-      MLIR
-      simp [State.drop_update_swap, h]
-      unfold State.dropFelts Map.drop State.updateFelts
-      aesop
+    Γ (Γ st ⟦@MLIR.DropFelt α y⟧) ⟦@MLIR.Assign β x (Op.Mul lhs rhs)⟧ =
+    Γ (Γ st ⟦@MLIR.Assign β x (Op.Mul lhs rhs)⟧) ⟦@MLIR.DropFelt α y⟧ := by
+      simp [MLIR.run_dropfelt, MLIR.run_ass_def, State.dropFelts, State.updateFelts, Map.drop_get h₂.symm , Map.drop_get h₁.symm, Map.update_drop_swap, *]
   
-  lemma drop_past_mul_nondet (h : ⟨x⟩ ≠ y) (h₁ : lhs ≠ y) (h₂ : rhs ≠ y) :
-    Γ st ⟦dropfelt y; nondet (x ←ₐ .Mul lhs rhs)⟧ =
-    Γ st ⟦nondet (x ←ₐ .Mul lhs rhs); dropfelt y⟧ := by
-      MLIR
-      simp [State.drop_update_swap, h]
-      unfold State.dropFelts Map.drop State.updateFelts
-      aesop
-
-  lemma drop_past_mul_single (h : ⟨x⟩ ≠ y) (h₁ : lhs ≠ y) (h₂ : rhs ≠ y):
-    Γ st ⟦@MLIR.DropFelt α y; x ←ₐ .Mul lhs rhs⟧ =
-    Γ st ⟦x ←ₐ .Mul lhs rhs; @MLIR.DropFelt α y⟧ := by
-      MLIR
-      simp [State.drop_update_swap, h]
-      unfold State.dropFelts Map.drop State.updateFelts
-      aesop
-  
-  lemma drop_past_set (h : y ≠ val) :
-    Γ st ⟦dropfelt y; .Set buf offset val⟧ =
-    Γ st ⟦.Set buf offset val; dropfelt y⟧ := by
-      MLIR; simp only [getElem!, dite_true, ne_eq]
-      rw [State.get_dropFelts_of_ne h]
-      unfold State.dropFelts Map.drop
-      simp only [
-        State.set!_felts, State.set!, State.setBufferElementImpl, Buffer.set?,
-        Buffer.getBufferAtTime!, Buffer.Idx.time, Buffer.Idx.data
-      ]
-      aesop
-  
-  lemma drop_past_set_nondet (h : val ≠ y) :
-    Γ st ⟦dropfelt y; nondet (.Set buf offset val)⟧ =
-    Γ st ⟦nondet( .Set buf offset val); dropfelt y⟧ := by
+  lemma drop_past_set (h : val ≠ y) :
+    Γ (Γ st ⟦@MLIR.DropFelt α y⟧) ⟦@MLIR.Set buf offset val⟧ =
+    Γ (Γ st ⟦@MLIR.Set buf offset val⟧) ⟦@MLIR.DropFelt α y⟧ := by
+      simp [MLIR.run_dropfelt, MLIR.run_set_def]
       MLIR; simp only [getElem!, dite_true, ne_eq]
       rw [State.get_dropFelts_of_ne h.symm]
       unfold State.dropFelts Map.drop
@@ -242,235 +235,161 @@ section drop
       aesop
 
   lemma drop_past_sub (h : ⟨x⟩ ≠ y) (h₁ : lhs ≠ y) (h₂ : rhs ≠ y) :
-    (Γ st ⟦@MLIR.DropFelt α y; x ←ₐ .Sub lhs rhs⟧) =
-    (Γ st ⟦x ←ₐ .Sub lhs rhs; @MLIR.DropFelt α y⟧) := by
-      MLIR
-      simp [State.drop_update_swap, h]
-      unfold State.dropFelts Map.drop State.updateFelts
-      aesop
-
-  lemma drop_past_nondet :
-    Γ st ⟦dropfelt y; nondet(prog)⟧ =
-    Γ st ⟦nondet(dropfelt y; prog)⟧ := by
-    MLIR
+    Γ (Γ st ⟦@MLIR.DropFelt α y⟧) ⟦@MLIR.Assign β x (Op.Sub lhs rhs)⟧ =
+    Γ (Γ st ⟦@MLIR.Assign β x (Op.Sub lhs rhs)⟧) ⟦@MLIR.DropFelt α y⟧ := by
+      sorry
 
 end drop
 
 section get
   lemma get_past_add (h: x ≠ y) (hl: ⟨x⟩ ≠ l) (hr: ⟨x⟩ ≠ r):
-    State.buffers (Γ st ⟦x ←ₐ .Get buf back offset; y ←ₐ .Add l r; rest⟧) =
-    State.buffers (Γ st ⟦y ←ₐ .Add l r; x ←ₐ .Get buf back offset; rest⟧) := by
-      MLIR
+    Γ (Γ st ⟦@MLIR.Assign α x (Op.Get buf back offset)⟧) ⟦@MLIR.Assign β y (Op.Add l r)⟧ =
+    Γ (Γ st ⟦@MLIR.Assign β y (Op.Add l r)⟧) ⟦@MLIR.Assign α x (Op.Get buf back offset)⟧ := by
+      simp only [MLIR.run_ass_def, Op.eval, *]
       generalize eq: getImpl st buf back offset = get
       cases get with
         | none => aesop
         | some lit =>
           have h_lit: ∃ k, lit = Lit.Val k := getImpl_val_of_some eq
-          aesop
-          rewrite [updateFelts_neq_comm]
-          rfl
-          simp [h]
+          sorry
+    
+  lemma get_past_andEqz (h: x ≠ y) (hl: ⟨x⟩ ≠ l) (hr: ⟨x⟩ ≠ r):
+    Γ (Γ st ⟦@MLIR.Assign α x (Op.Get buf back offset)⟧) ⟦@MLIR.Assign β y (Op.AndEqz l r)⟧ =
+    Γ (Γ st ⟦@MLIR.Assign β y (Op.AndEqz l r)⟧) ⟦@MLIR.Assign α x (Op.Get buf back offset)⟧ := by
+      simp only [MLIR.run_ass_def, Op.eval, *]
+      generalize eq: getImpl st buf back offset = get
+      cases get with
+        | none => aesop
+        | some lit =>
+          have h_lit: ∃ k, lit = Lit.Val k := getImpl_val_of_some eq
+          sorry
 
-  lemma get_past_bitAnd_nondet (h: x ≠ y) (hl: ⟨x⟩ ≠ l) (hr: ⟨x⟩ ≠ r):
-    State.buffers (Γ st ⟦x ←ₐ .Get buf back offset; nondet(y ←ₐ .BitAnd l r; s₁); s₂⟧) =
-    State.buffers (Γ st ⟦nondet (y ←ₐ .BitAnd l r); x ←ₐ .Get buf back offset; nondet s₁; s₂⟧) := by
-      MLIR
-      generalize eq: getImpl st buf back offset = get
-      cases get with
-        | none => aesop
-        | some lit =>
-          have h_lit: ∃ k, lit = Lit.Val k := getImpl_val_of_some eq
-          aesop
-          rewrite [updateFelts_neq_comm]
-          rfl
-          simp [h]
-
-  lemma get_past_bitAnd_nondet_single (h: x ≠ y) (hl: ⟨x⟩ ≠ l) (hr: ⟨x⟩ ≠ r):
-    State.buffers (Γ st ⟦x ←ₐ .Get buf back offset; nondet(y ←ₐ .BitAnd l r); s₂⟧) =
-    State.buffers (Γ st ⟦nondet (y ←ₐ .BitAnd l r); x ←ₐ .Get buf back offset; s₂⟧) := by
-      MLIR
-      generalize eq: getImpl st buf back offset = get
-      cases get with
-        | none => aesop
-        | some lit =>
-          have h_lit: ∃ k, lit = Lit.Val k := getImpl_val_of_some eq
-          aesop
-          rewrite [updateFelts_neq_comm]
-          rfl
-          simp [h]
+  lemma get_past_bitAnd (h: x ≠ y) (hl: ⟨x⟩ ≠ l) (hr: ⟨x⟩ ≠ r):
+    Γ (Γ st ⟦@MLIR.Assign α x (Op.Get buf back offset)⟧) ⟦@MLIR.Assign β y (Op.BitAnd l r)⟧ =
+    Γ (Γ st ⟦@MLIR.Assign β y (Op.BitAnd l r)⟧) ⟦@MLIR.Assign α x (Op.Get buf back offset)⟧ := by
+      sorry
 
   lemma get_past_const (h: x ≠ y) :
-  State.buffers (Γ st ⟦x ←ₐ .Get buf back offset; y ←ₐ C c; rest⟧) =
-  State.buffers (Γ st ⟦y ←ₐ C c; x ←ₐ .Get buf back offset; rest⟧) := by
-    MLIR
-    generalize eq: getImpl st buf back offset = get
-    cases get with
-      | none => aesop
-      | some lit =>
-        have h_lit: ∃ k, lit = Lit.Val k := getImpl_val_of_some eq
-        aesop
-        rewrite [updateFelts_neq_comm]
-        rfl
-        simp [h]
+  Γ (Γ st ⟦@MLIR.Assign α x (Op.Get buf back offset)⟧) ⟦@MLIR.Assign β y (Op.Const c)⟧ =
+  Γ (Γ st ⟦@MLIR.Assign β y (Op.Const c)⟧) ⟦@MLIR.Assign α x (Op.Get buf back offset)⟧ := by
+    rewrite [const_past_get] <;> aesop
+    
 
-  lemma get_past_drop (h: ⟨x⟩ ≠ y) :
-  State.buffers (Γ st ⟦x ←ₐ .Get buf back offset; dropfelt y; rest⟧) =
-  State.buffers (Γ st ⟦dropfelt y; x ←ₐ .Get buf back offset; rest⟧) := by
-    MLIR
-    generalize eq: getImpl st buf back offset = get
-    cases get with
-      | none => aesop
-      | some lit =>
-        have h_lit: ∃ k, lit = Lit.Val k := getImpl_val_of_some eq
-        aesop
+  -- lemma get_past_drop (h: ⟨x⟩ ≠ y) :
+  -- Γ st ⟦@MLIR.Assign x .Get buf back offset⟧) ⟦dropfelt y⟧ =
+  -- Γ st ⟦dropfelt y⟧) ⟦@MLIR.Assign x .Get buf back offset⟧ := by
+  --   MLIR
+  --   generalize eq: getImpl st buf back offset = get
+  --   cases get with
+  --     | none => aesop
+  --     | some lit =>
+  --       have h_lit: ∃ k, lit = Lit.Val k := getImpl_val_of_some eq
+  --       aesop
 
-  lemma get_past_mul (h: x ≠ y) (hl: ⟨x⟩ ≠ l) (hr: ⟨x⟩ ≠ r):
-    State.buffers (Γ st ⟦x ←ₐ .Get buf back offset; y ←ₐ .Mul l r; rest⟧) =
-    State.buffers (Γ st ⟦y ←ₐ .Mul l r; x ←ₐ .Get buf back offset; rest⟧) := by
-      MLIR
-      generalize eq: getImpl st buf back offset = get
-      cases get with
-        | none => aesop
-        | some lit =>
-          have h_lit: ∃ k, lit = Lit.Val k := getImpl_val_of_some eq
-          aesop
-          rewrite [updateFelts_neq_comm]
-          rfl
-          simp [h]
-
-  lemma get_past_mul_nondet (h: x ≠ y) (hl: ⟨x⟩ ≠ l) (hr: ⟨x⟩ ≠ r):
-    State.buffers (Γ st ⟦x ←ₐ .Get buf back offset; nondet(y ←ₐ .Mul l r; s₁); s₂⟧) =
-    State.buffers (Γ st ⟦nondet (y ←ₐ .Mul l r); x ←ₐ .Get buf back offset; nondet s₁; s₂⟧) := by
-      MLIR
-      generalize eq: getImpl st buf back offset = get
-      cases get with
-        | none => aesop
-        | some lit =>
-          have h_lit: ∃ k, lit = Lit.Val k := getImpl_val_of_some eq
-          aesop
-          rewrite [updateFelts_neq_comm]
-          rfl
-          simp [h]
 
   lemma get_past_get_buf (h: buf ≠ buf') (h': x ≠ y) :
-    State.buffers (Γ st ⟦x ←ₐ .Get buf back offset; y ←ₐ .Get buf' back' offset'; rest⟧) =
-    State.buffers (Γ st ⟦y ←ₐ .Get buf' back' offset';x ←ₐ .Get buf back offset;  rest⟧) := by
-      MLIR
-      generalize eq1: getImpl st buf back offset = get1
-      generalize eq2: getImpl st buf' back' offset' = get2
-      cases get1 with
-        | none => simp [State.update]; aesop
-        | some lit1 =>
-          have h1: ∃ k1, lit1 = Lit.Val k1 := getImpl_val_of_some eq1
-          cases get2 with
-            | none => aesop
-            | some lit2 =>
-              have h2: ∃ k2, lit2 = Lit.Val k2 := getImpl_val_of_some eq2
-              aesop
-              rewrite [updateFelts_neq_comm]
-              rfl
-              simp [h']
+    Γ (Γ st ⟦@MLIR.Assign α x (Op.Get buf back offset)⟧) ⟦@MLIR.Assign β y (Op.Get buf' back' offset')⟧ =
+    Γ (Γ st ⟦@MLIR.Assign β y (Op.Get buf' back' offset')⟧) ⟦@MLIR.Assign α x (Op.Get buf back offset)⟧ := by
+      sorry
 
   lemma get_past_get_offset (h: offset ≠ offset') (h': x ≠ y) :
-    State.buffers (Γ st ⟦x ←ₐ .Get buf back offset; y ←ₐ .Get buf' back' offset'; rest⟧) =
-    State.buffers (Γ st ⟦y ←ₐ .Get buf' back' offset';x ←ₐ .Get buf back offset;  rest⟧) := by
-      MLIR
+    Γ (Γ st ⟦@MLIR.Assign α x (Op.Get buf back offset)⟧) ⟦@MLIR.Assign β y (Op.Get buf' back' offset')⟧ =
+    Γ (Γ st ⟦@MLIR.Assign β y (Op.Get buf' back' offset')⟧) ⟦@MLIR.Assign α x (Op.Get buf back offset)⟧ := by
+      simp only [MLIR.run_ass_def, Op.eval] --REVIEW: eval_getBuffer does not go to getImpl, is this expected
       generalize eq1: getImpl st buf back offset = get1
       generalize eq2: getImpl st buf' back' offset' = get2
-      cases get1 with
-        | none => simp [State.update]; aesop
-        | some lit1 =>
-          have h1: ∃ k1, lit1 = Lit.Val k1 := getImpl_val_of_some eq1
-          cases get2 with
-            | none => aesop
-            | some lit2 =>
-              have h2: ∃ k2, lit2 = Lit.Val k2 := getImpl_val_of_some eq2
-              aesop
-              rewrite [updateFelts_neq_comm]
-              rfl
-              simp [h']
+      sorry
 
-  lemma get_past_set_buf_nondet (h: ⟨x⟩ ≠ val) (h': buf' ≠ buf):
-    State.buffers (Γ st ⟦x ←ₐ .Get buf back offset; nondet(buf'[index] ←ᵢ val; s₁); s₂⟧) =
-    State.buffers (Γ st ⟦nondet (buf'[index] ←ᵢ val); x ←ₐ .Get buf back offset; nondet s₁; s₂⟧) := by
-      MLIR
+  lemma get_past_mul (h: x ≠ y) (hl: ⟨x⟩ ≠ l) (hr: ⟨x⟩ ≠ r):
+    Γ (Γ st ⟦@MLIR.Assign α x (Op.Get buf back offset)⟧) ⟦@MLIR.Assign β y (Op.Mul l r)⟧ =
+    Γ (Γ st ⟦@MLIR.Assign β y (Op.Mul l r)⟧) ⟦@MLIR.Assign α x (Op.Get buf back offset)⟧ := by
+      simp only [MLIR.run_ass_def, Op.eval, *]
       generalize eq: getImpl st buf back offset = get
       cases get with
-        | none => sorry
-        | some lit1 => sorry
+        | none => aesop
+        | some lit =>
+          have h_lit: ∃ k, lit = Lit.Val k := getImpl_val_of_some eq
+          sorry
 
-  lemma get_past_set_buf_nondet_single (h: ⟨x⟩ ≠ val) (h': buf' ≠ buf):
-    State.buffers (Γ st ⟦x ←ₐ .Get buf back offset; nondet(buf'[index] ←ᵢ val); s₂⟧) =
-    State.buffers (Γ st ⟦nondet (buf'[index] ←ᵢ val); x ←ₐ .Get buf back offset; s₂⟧) := by
-      MLIR
+  lemma get_past_set_buf (h: ⟨x⟩ ≠ val) (h': buf' ≠ buf):
+    Γ (Γ st ⟦@MLIR.Assign α x (Op.Get buf back offset)⟧) ⟦@MLIR.Set buf' index val⟧ =
+    Γ (Γ st ⟦@MLIR.Set buf' index val⟧) ⟦@MLIR.Assign α x (Op.Get buf back offset)⟧ := by
+      sorry
+
+  lemma get_past_sub (h: x ≠ y) (hl: ⟨x⟩ ≠ l) (hr: ⟨x⟩ ≠ r):
+    Γ (Γ st ⟦@MLIR.Assign α x (Op.Get buf back offset)⟧) ⟦@MLIR.Assign β y (Op.Sub l r)⟧ =
+    Γ (Γ st ⟦@MLIR.Assign β y (Op.Sub l r)⟧) ⟦@MLIR.Assign α x (Op.Get buf back offset)⟧ := by
+      simp only [MLIR.run_ass_def, Op.eval, *]
       generalize eq: getImpl st buf back offset = get
       cases get with
-        | none => sorry
-        | some lit1 => sorry
+        | none => aesop
+        | some lit =>
+          have h_lit: ∃ k, lit = Lit.Val k := getImpl_val_of_some eq
+          sorry
 
 end get
 
 section inv
-  lemma drop_assign_inv_swap (h : name ≠ name') (h₁ : ⟨name'⟩ ≠ lhs) :
-    Γ st ⟦name ←ₐ .Inv lhs; dropfelt ⟨name'⟩⟧ =
-    Γ st ⟦dropfelt ⟨name'⟩; name ←ₐ .Inv lhs⟧ := by
-      MLIR
-      simp [State.drop_update_swap, h, State.get_dropFelts_of_ne h₁]
+  -- lemma drop_assign_inv_swap (h : name ≠ name') (h₁ : ⟨name'⟩ ≠ lhs) :
+  --   Γ (Γ st ⟦@MLIR.Assign name .Inv lhs⟧) ⟦dropfelt ⟨name'⟩⟧ =
+  --   Γ (Γ st ⟦dropfelt ⟨name'⟩⟧) ⟦@MLIR.Assign name .Inv lhs⟧ := by
+  --     MLIR
+  --     simp [State.drop_update_swap, h, State.get_dropFelts_of_ne h₁]
 end inv
 
 section isz
-  lemma drop_assign_isz_swap (h : name ≠ name') (h₁ : ⟨name'⟩ ≠ lhs) :
-    Γ st ⟦name ←ₐ .Isz lhs; dropfelt ⟨name'⟩⟧ =
-    Γ st ⟦dropfelt ⟨name'⟩; name ←ₐ .Isz lhs⟧ := by
-      MLIR
-      simp [State.drop_update_swap, h]
-      unfold State.dropFelts Map.drop State.updateFelts
-      aesop
+  -- lemma drop_assign_isz_swap (h : name ≠ name') (h₁ : ⟨name'⟩ ≠ lhs) :
+  --   Γ (Γ st ⟦@MLIR.Assign name .Isz lhs⟧) ⟦dropfelt ⟨name'⟩⟧ =
+  --   Γ (Γ st ⟦dropfelt ⟨name'⟩⟧) ⟦@MLIR.Assign name .Isz lhs⟧ := by
+  --     MLIR
+  --     simp [State.drop_update_swap, h]
+  --     unfold State.dropFelts Map.drop State.updateFelts
+  --     aesop
 end isz
 
 section mul
-  lemma mul_past_drop (h : name ≠ name') (h₁ : ⟨name'⟩ ≠ lhs) (h₂ : ⟨name'⟩ ≠ rhs):
-    Γ st ⟦name ←ₐ .Mul lhs rhs; @MLIR.DropFelt α ⟨name'⟩⟧ =
-    Γ st ⟦@MLIR.DropFelt α ⟨name'⟩; name ←ₐ .Mul lhs rhs⟧ := by
-      MLIR
-      simp [State.drop_update_swap, h]
-      unfold State.dropFelts Map.drop State.updateFelts
-      aesop
+  -- lemma mul_past_drop (h : name ≠ name') (h₁ : ⟨name'⟩ ≠ lhs) (h₂ : ⟨name'⟩ ≠ rhs):
+  --   Γ (Γ st ⟦@MLIR.Assign name .Mul lhs rhs⟧) ⟦@MLIR.DropFelt α ⟨name'⟩⟧ =
+  --   Γ (Γ st ⟦@MLIR.DropFelt α ⟨name'⟩⟧) ⟦@MLIR.Assign name .Mul lhs rhs⟧ := by
+  --     MLIR
+  --     simp [State.drop_update_swap, h]
+  --     unfold State.dropFelts Map.drop State.updateFelts
+  --     aesop
 end mul
 
 section neg
-  lemma neg_past_drop (h : name ≠ name') (h₁ : ⟨name'⟩ ≠ lhs):
-    Γ st ⟦name ←ₐ .Neg lhs; @MLIR.DropFelt α ⟨name'⟩⟧ =
-    Γ st ⟦@MLIR.DropFelt α ⟨name'⟩; name ←ₐ .Neg lhs⟧ := by
-      MLIR
-      simp [State.drop_update_swap, h]
-      unfold State.dropFelts Map.drop
-      aesop
+  -- lemma neg_past_drop (h : name ≠ name') (h₁ : ⟨name'⟩ ≠ lhs):
+  --   Γ (Γ st ⟦@MLIR.Assign name .Neg lhs⟧) ⟦@MLIR.DropFelt α ⟨name'⟩⟧ =
+  --   Γ (Γ st ⟦@MLIR.DropFelt α ⟨name'⟩⟧) ⟦@MLIR.Assign name .Neg lhs⟧ := by
+  --     MLIR
+  --     simp [State.drop_update_swap, h]
+  --     unfold State.dropFelts Map.drop
+  --     aesop
 end neg
 
 section pow
-  lemma drop_assign_pow_swap {n : ℕ} (h : name ≠ name') (h₁ : ⟨name'⟩ ≠ lhs) :
-    Γ st ⟦name ←ₐ .Pow lhs n; @MLIR.DropFelt α ⟨name'⟩⟧ =
-    Γ st ⟦@MLIR.DropFelt α ⟨name'⟩; name ←ₐ .Pow lhs n⟧ := by
-      MLIR
-      simp [State.drop_update_swap, h, State.get_dropFelts_of_ne' h₁]
+  -- lemma drop_assign_pow_swap {n : ℕ} (h : name ≠ name') (h₁ : ⟨name'⟩ ≠ lhs) :
+  --   Γ (Γ st ⟦@MLIR.Assign name .Pow lhs n⟧) ⟦@MLIR.DropFelt α ⟨name'⟩⟧ =
+  --   Γ (Γ st ⟦@MLIR.DropFelt α ⟨name'⟩⟧) ⟦@MLIR.Assign name .Pow lhs n⟧ := by
+  --     MLIR
+  --     simp [State.drop_update_swap, h, State.get_dropFelts_of_ne' h₁]
 end pow
 
 section sub
-  lemma sub_past_drop (h : name ≠ name') (h₁ : ⟨name'⟩ ≠ lhs) (h₂ : ⟨name'⟩ ≠ rhs):
-    Γ st ⟦name ←ₐ .Sub lhs rhs; @MLIR.DropFelt α ⟨name'⟩⟧ =
-    Γ st ⟦@MLIR.DropFelt α ⟨name'⟩; name ←ₐ .Sub lhs rhs⟧ := by
-      MLIR
-      simp [State.drop_update_swap, h]
-      unfold State.dropFelts Map.drop State.updateFelts
-      aesop
+  -- lemma sub_past_drop (h : name ≠ name') (h₁ : ⟨name'⟩ ≠ lhs) (h₂ : ⟨name'⟩ ≠ rhs):
+  --   Γ (Γ st ⟦@MLIR.Assign name .Sub lhs rhs⟧) ⟦@MLIR.DropFelt α ⟨name'⟩⟧ =
+  --   Γ (Γ st ⟦@MLIR.DropFelt α ⟨name'⟩⟧) ⟦@MLIR.Assign name .Sub lhs rhs⟧ := by
+  --     MLIR
+  --     simp [State.drop_update_swap, h]
+  --     unfold State.dropFelts Map.drop State.updateFelts
+  --     aesop
 end sub
 
 section true
   -- lemma drop_assign_true_swap {α : IsNondet} {name name' : String} {x : Felt}
   --   (h : name ≠ name') :
-  --   Γ st ⟦name ←ₐ ⊤; @MLIR.DropFelt α ⟨name'⟩⟧ =
-  --   Γ st ⟦@MLIR.DropFelt α ⟨name'⟩; name ←ₐ ⊤⟧ := by
+  --   Γ st ⟦@MLIR.Assign name ⊤⟧) ⟦@MLIR.DropFelt α ⟨name'⟩⟧ =
+  --   Γ st ⟦@MLIR.DropFelt α ⟨name'⟩⟧) ⟦@MLIR.Assign name ⊤⟧ := by
   --   MLIR
   --   simp [State.drop_update_swap, h]
 end true
@@ -550,6 +469,22 @@ lemma drop_sequencing_nnnn :
   Γ st ⟦nondet (s₁; s₂; s₃; s₄)⟧ = Γ (Γ (Γ (Γ st ⟦s₁⟧) ⟦s₂⟧) ⟦s₃⟧) ⟦s₄⟧ :=
   by aesop
 
+lemma drop_sequencing_ddd:
+  Γ st ⟦@MLIR.DropFelt .NotInNondet x; s₁; s₂⟧ = Γ (Γ (Γ st ⟦@MLIR.DropFelt .NotInNondet x⟧) ⟦s₁⟧) ⟦s₂⟧ :=
+  by aesop
+
+lemma drop_sequencing_dnd:
+  Γ st ⟦@MLIR.DropFelt .NotInNondet x; nondet s₁; s₂⟧ = Γ (Γ (Γ st ⟦@MLIR.DropFelt .NotInNondet x⟧) ⟦s₁⟧) ⟦s₂⟧ :=
+  by aesop
+
+lemma drop_sequencing_ddn:
+  Γ st ⟦@MLIR.DropFelt .NotInNondet x; s₁; nondet s₂⟧ = Γ (Γ (Γ st ⟦@MLIR.DropFelt .NotInNondet x⟧) ⟦s₁⟧) ⟦s₂⟧ :=
+  by aesop
+
+lemma drop_sequencing_dnn:
+  Γ st ⟦@MLIR.DropFelt .NotInNondet x; nondet (s₁; s₂)⟧ = Γ (Γ (Γ st ⟦@MLIR.DropFelt .NotInNondet x⟧) ⟦s₁⟧) ⟦s₂⟧ :=
+  by aesop
+
 lemma drop_sequencing_dd:
   Γ st ⟦@MLIR.DropFelt .NotInNondet x; s₁⟧ = Γ (Γ st ⟦@MLIR.DropFelt .NotInNondet x⟧) ⟦s₁⟧ :=
   by aesop
@@ -557,6 +492,13 @@ lemma drop_sequencing_dd:
 lemma drop_sequencing_dn:
   Γ st ⟦@MLIR.DropFelt .NotInNondet x; nondet s₁⟧ = Γ (Γ st ⟦@MLIR.DropFelt .NotInNondet x⟧) ⟦s₁⟧ :=
   by aesop
+
+lemma drop_sequencing_d:
+  Γ st ⟦@MLIR.DropFelt .NotInNondet x⟧ = Γ st ⟦@MLIR.DropFelt .NotInNondet x⟧ := rfl
+
+-- TODO general tactic for unrolling N statements regardless of det/nondet like this would be nice
+-- alternatively, process out nondet blocks up front
+
 end drop_sequencing
 
 end Reordering
